Blanc.lean
@@ -140,6 +140,7 @@ import Blanc.ProxyPairOssifiableConstructor
 import Blanc.ProxyPairOssifiableConstructorDecode
 import Blanc.ProxyPairOssifiableConstructorInitialize
 import Blanc.ProxyPairOssifiableConstructorEffects
+import Blanc.ProxyPairOssifiableConstructorSetup
 import Blanc.ProxyPairImplementation
 import Blanc.ProxyPairExecution
 import Blanc.ProxyPairCorrespondence
